opex:Unit a owl:Class ;
    rdfs:label "Unit"^^xsd:string ;
    rdfs:isDefinedBy <http://openpermissions.org/ns/opex/1.0/> .

opex:UnitScheme a skos:ConceptScheme ;
    skos:hasTopConcept opex:topUnit .

opex:topUnit a opex:Unit,
        skos:Concept ;
    skos:inScheme opex:UnitScheme ;
    rdfs:label "topUnit"@en .

opex:pixel a opex:Unit,
        skos:Concept ;
    skos:inScheme opex:UnitScheme ;
    rdfs:label "pixel"@en ;
    skos:narrowerThan opex:topUnit .

opex:visitorsPerMonth a opex:Unit,
        skos:Concept ;
    skos:inScheme opex:UnitScheme ;
    rdfs:label "visitorsPerMonth"@en ;
    skos:narrowerThan opex:topUnit .

opex:attributeText a owl:DatatypeProperty,
        owl:FunctionalProperty ;
    rdfs:label """Attribute Text"""@en ;
    rdfs:comment """Required textual representation of copyrights attribution."""@en ;
    rdfs:domain opex:Constraint ;
    rdfs:isDefinedBy <http://openpermissions.org/ns/opex/1.0/> ;
    rdfs:range xsd:string ;
    rdfs:subPropertyOf odrl:rightOperand .

opex:height a owl:DatatypeProperty,
        owl:FunctionalProperty ;
    rdfs:comment """Specifies the vertical height of the asset."""@en ;
    rdfs:label """height"""@en ;
    rdfs:domain opex:Constraint ;
    rdfs:isDefinedBy <http://openpermissions.org/ns/opex/1.0/> ;
    rdfs:range xsd:decimal ;
    rdfs:subPropertyOf odrl:rightOperand .

opex:width a owl:DatatypeProperty,
        owl:FunctionalProperty ;
    rdfs:comment """Specifies the horizontal width of the asset."""@en ;
    rdfs:label """width"""@en ;
    rdfs:domain opex:Constraint ;
    rdfs:isDefinedBy <http://openpermissions.org/ns/opex/1.0/> ;
    rdfs:range xsd:decimal ;
    rdfs:subPropertyOf odrl:rightOperand .

opex:host a owl:FunctionalProperty,
        owl:ObjectProperty ;
    rdfs:label """host"""@en ;
    rdfs:comment """Specifies on which type of host the asset may be presented or posted."""@en ;
    rdfs:domain opex:Constraint ;
    rdfs:isDefinedBy <http://openpermissions.org/ns/opex/1.0/> ;
    rdfs:range opex:Host ;
    rdfs:subPropertyOf odrl:rightOperand .

opex:views a owl:DatatypeProperty,
        owl:FunctionalProperty ;
    rdfs:label """views"""@en ;
    rdfs:comment """Specifies the maximum number of views of the asset that may result in."""@en ;
    rdfs:domain opex:Constraint ;
    rdfs:isDefinedBy <http://openpermissions.org/ns/opex/1.0/> ;
    rdfs:range xsd:integer ;
    rdfs:subPropertyOf odrl:rightOperand .

opex:Constraint a owl:Class ;
    rdfs:subClassOf odrl:Constraint,
        [ a owl:Restriction ;
            owl:maxCardinality 1 ;
            owl:onProperty opex:views ],
        [ a owl:Restriction ;
            owl:maxCardinality 1 ;
            owl:onProperty opex:height ],
        [ a owl:Restriction ;
            owl:allValuesFrom opex:Host ;
            owl:maxCardinality 1 ;
            owl:onProperty opex:host ],
        [ a owl:Restriction ;
            owl:maxCardinality 1 ;
            owl:onProperty opex:width ],
        [ a owl:Restriction ;
            owl:maxCardinality 1 ;
            owl:onProperty opex:attributeText ] ;
    rdfs:label "Constraint"^^xsd:string ;
    rdfs:isDefinedBy <http://openpermissions.org/ns/opex/1.0/> .

opex:Host a owl:Class ;
    rdfs:comment """The Host describes the type of site or device the asset can be used on."""@en ;
    rdfs:label "Host"^^xsd:string ;
    rdfs:isDefinedBy <http://openpermissions.org/ns/opex/1.0/> .

opex:HostScheme a skos:ConceptScheme ;
    skos:hasTopConcept opex:anyHost .

opex:anyHost a opex:Host,
    skos:Concept ;
    skos:inScheme opex:HostScheme ;
    rdfs:label "anyHost"@en .

opex:personalDevice a opex:Host,
        skos:Concept ;
    rdfs:comment """The Asset can be used on personal devices (e.g: Mobile Phone, Desktop Background, Camera Roll)"""@en ;
    skos:inScheme opex:HostScheme ;
    rdfs:label "personal device"@en ;
    skos:narrowerThan opex:anyHost .

opex:personalSocialMediaWebsite a opex:Host,
        skos:Concept ;
    rdfs:comment """The Asset can be used on personal social media accounts."""@en ;
    skos:inScheme opex:HostScheme ;
    rdfs:label "personal social media site"@en ;
    skos:narrowerThan opex:anyHost .

opex:nonCommercialWebsite a opex:Host,
        skos:Concept ;
    rdfs:comment """The Asset can be used on a personal website that does not generate income or carry advertising."""@en ;
    skos:inScheme opex:HostScheme ;
    rdfs:label "non commercial website"@en ;
    skos:narrowerThan opex:anyHost .

opex:commercialWebsite a opex:Host,
        skos:Concept ;
    rdfs:comment """The Asset can be used on a website that generates income or carries advertising."""@en ;
    skos:inScheme opex:HostScheme ;
    rdfs:label "commercial website"@en ;
    skos:narrowerThan opex:anyHost .

