op:alsoIdentifiedBy a owl:ObjectProperty ;
    rdfs:comment """An Asset may have different identifiers assigned to it.
    The identities are not necessarily equivalent even though they have been assigned to the same Asset.
    Each identity has a type, such as ISBN or EIDR and the type is semantically defined.
    Identities that alsoIdentifiedBy refer to MUST be for the whole Asset and not for part of the Asset.
    For example if the Asset is a book, the alsoIdentifiedBy ids will be for the book and NOT for pictures in the book."""@en ;
    rdfs:domain op:Asset ;
    rdfs:isDefinedBy <http://openpermissions.org/ns/op/1.1/> ;
    rdfs:range op:Id .

op:title a owl:DatatypeProperty,
        owl:FunctionalProperty ;
    rdfs:comment """Title of the Asset for the purpose of presentation to a Licensee."""@en ;
    rdfs:domain op:Asset ;
    rdfs:isDefinedBy <http://openpermissions.org/ns/op/1.1/> ;
    rdfs:range xsd:string ;
    rdfs:subPropertyOf dc:title .

op:Asset a owl:Class ;
    rdfs:subClassOf odrl:Asset ,
        [ a owl:Restriction ;
            owl:maxCardinality 1 ;
            owl:onProperty op:title ],
        [ a owl:Restriction ;
            owl:allValuesFrom op:Id ;
            owl:onProperty op:alsoIdentifiedBy ] ;
    rdfs:label "Asset"^^xsd:string ;
    rdfs:comment """An Asset in ODRL is any object referred by a policy.
    Here the Asset generally represents the intellectual work.
    Only metadata about the Asset that is required for the licensing of the Asset should be defined here."""@en ;
    rdfs:isDefinedBy <http://openpermissions.org/ns/op/1.1/> .
