op:name a owl:DatatypeProperty,
        owl:FunctionalProperty ;
    rdfs:domain op:Party ;
    rdfs:isDefinedBy <http://openpermissions.org/ns/op/1.1/> ;
    rdfs:range xsd:string ;
    rdfs:subPropertyOf dc:name .

op:provider a owl:DatatypeProperty,
        owl:FunctionalProperty ;
    rdfs:comment """
origanisation_id of the organisation representing the party.
if no value is provider the party is the organisation itself
"""@en ;
    rdfs:domain op:Party ;
    rdfs:isDefinedBy <http://openpermissions.org/ns/op/1.1/> ;
    rdfs:range xsd:string .

op:reference a owl:DatatypeProperty,
        owl:FunctionalProperty ;
    rdfs:domain op:Party ;
    rdfs:isDefinedBy <http://openpermissions.org/ns/op/1.1/> ;
    rdfs:range xsd:string ;
    rdfs:subPropertyOf dc:source ;
    rdfs:comment """An reference id used by the provider to actually identify the party"""@en .

op:Party a owl:Class ;
    rdfs:subClassOf op:Asset,
        odrl:Party,
        [ a owl:Restriction ;
            owl:maxCardinality 1 ;
            owl:onProperty op:reference ],
        [ a owl:Restriction ;
            owl:maxCardinality 1 ;
            owl:onProperty op:provider ],
        [ a owl:Restriction ;
            owl:maxCardinality 1 ;
            owl:onProperty op:name ] ;
    rdfs:label "Party"^^xsd:string ;
    rdfs:comment """
A party represent:
  1. a legal person having duties and permissions as part of agreements.
  2. a person known by an organisation (not necessarily providing its real name)
"""@en ;
    rdfs:isDefinedBy <http://openpermissions.org/ns/op/1.1/> .

